prove some progress lemmas, fix Ctx

LocalLang/TypingGuarantees.lean
@@ -6,16 +6,13 @@ import LocalLang.Typing
 def EnvRespectsCtx (Γ : TypeContext) (V : Env) : Prop := sorry
 
 def CtxRespectsEnv (V : Env) (Γ : TypeContext) : Prop :=
-  sorry
+  ∀ (x : String) (ty : LLType), Γ[x]? = some ty
+  → ∃ v, V[x]? = some v ∧ v.TypeJdg ty
 
 inductive IsFuncType : LLType → Prop where
   | func {param_tys ret_ty} : IsFuncType (.func param_tys ret_ty)
 
--- def CtxRespectsDefs (defs : Definitions) (Γ : TypeContext) : Prop :=
---   sorry
-
 -- TODO: prove
--- TODO: V and Γ should be related
 theorem preservation (Γ : TypeContext) (e e' : Expr) (ty : LLType)
     (h_env_respects : EnvRespectsCtx Γ V)
   : Expr.TypeJdg Γ e ty → HeadSmallStep V e e' → Expr.TypeJdg Γ e' ty := sorry
@@ -29,7 +26,7 @@ def Expr.simple_rec.{l} {motive : Expr → Sort l}
      (var_case : ∀ x, motive (.var x))
      (bin_op_case : ∀ op lhs rhs, motive lhs → motive rhs → motive (.binOp op lhs rhs))
      (let_in_case : ∀ name e₁ e₂, motive e₁ → motive e₂ → motive (.letIn name e₁ e₂))
-     (fun_case : ∀ f es, (∀ e', e' ∈ es → motive e') → motive (.funCall f es))
+     (fun_case : ∀ f es, motive f → (∀ e', e' ∈ es → motive e') → motive (.funCall f es))
     : (e : Expr) → motive e := go
 where go
   | .value v => value_case v
@@ -37,31 +34,138 @@ where go
   | .var x => var_case x
   | .binOp op lhs rhs => bin_op_case op lhs rhs (go lhs) (go rhs)
   | .letIn name e₁ e₂ => let_in_case name e₁ e₂ (go e₁) (go e₂)
-  | .funCall f es => fun_case f es (fun e' _ => go e')
+  | .funCall f es => fun_case f es (go f) (fun e' _ => go e')
 
-inductive IsConst : Expr → Prop where
-  | const : IsConst (.const n)
+inductive IsValue : Expr → Prop where
+  | value : IsValue (.value v)
 
 inductive IsRedex : Expr → Prop where
+  | const : IsRedex (.const n)
   | var : IsRedex (.var x)
-  | binOp {op} : IsRedex (.binOp op (.const n₁) (.const n₂))
-  | letInConst : IsRedex (.letIn x (.const n₁) (.const n₂))
-  | funCall {es} : IsRedex (.funCall f es)
+  | binOp {op} : IsRedex (.binOp op (.value v₁) (.value v₂))
+  | letInConst : IsRedex (.letIn x (.value v₁) (.value v₂))
+  | funCall {es} : IsRedex (.funCall (.value v) es)
 
 inductive HasDecomposition : Expr → Prop where
   | decomposition (e' : Expr) (ctx : Ctx) : e = ctx.fill e' → IsRedex e' → HasDecomposition e
 
-lemma is_const_or_has_decomposition : ∀ e : Expr, IsConst e ∨ HasDecomposition e := by
-  sorry
+lemma is_value_or_has_decomposition : ∀ e : Expr, IsValue e ∨ HasDecomposition e := by
+  intro e
+  apply e.simple_rec
+  · intro v
+    apply Or.intro_left
+    constructor
+  · intro n
+    apply Or.intro_right
+    apply HasDecomposition.decomposition (.const n) .hole (by simp)
+    constructor
+  · intro x
+    apply Or.intro_right
+    apply HasDecomposition.decomposition (.var x) .hole (by simp)
+    constructor
+  · intro op lhs rhs ih_lhs ih_rhs
+    apply Or.intro_right
+    cases ih_lhs with
+    | inl lhs_const =>
+      cases lhs_const
+      rename_i v₁
+      cases ih_rhs with
+      | inl rhs_const =>
+        cases rhs_const
+        rename_i v₂
+        apply HasDecomposition.decomposition (.binOp op (Expr.value v₁) (Expr.value v₂))
+          .hole (by simp)
+        constructor
+      | inr rhs_dec =>
+        let ⟨e', ctx, e_eq, e'_redex⟩ := rhs_dec
+        apply HasDecomposition.decomposition e' (.binOpRhs v₁ op ctx) (by simp [e_eq])
+        assumption
+    | inr lhs_dec =>
+      let ⟨e', ctx, e_eq, e'_redex⟩ := lhs_dec
+      apply HasDecomposition.decomposition e' (.binOpLhs ctx op rhs) (by simp [e_eq])
+      assumption
+  · intro name e₁ e₂ ih_e₁ ih_e₂
+    apply Or.intro_right
+    cases ih_e₁ with
+    | inl e₁_const =>
+      cases e₁_const
+      rename_i v₁
+      cases ih_e₂ with
+      | inl e₂_const =>
+        cases e₂_const
+        rename_i v₂
+        apply HasDecomposition.decomposition (Expr.letIn name (Expr.value v₁) (Expr.value v₂))
+          .hole (by simp)
+        constructor
+      | inr e₂_dec =>
+        let ⟨e', ctx, e_eq, e'_redex⟩ := e₂_dec
+        apply HasDecomposition.decomposition e' (.letInBody name v₁ ctx) (by simp [e_eq])
+        assumption
+    | inr e₁_dec =>
+      let ⟨e', ctx, e_eq, e'_redex⟩ := e₁_dec
+      apply HasDecomposition.decomposition e' (.letInExpr name ctx e₂) (by simp [e_eq])
+      assumption
+  · intro f es ih_f ih_es
+    apply Or.intro_right
+    cases ih_f
+    · rename_i f_value
+      cases f_value
+      rename_i v
+      apply HasDecomposition.decomposition ((Expr.value v).funCall es) .hole (by simp)
+      constructor
+    · rename_i f_dec
+      let ⟨e', ctx, fill_eq, e'_redex⟩ := f_dec
+      apply HasDecomposition.decomposition e' (.funCallBody ctx es) (by simp [fill_eq])
+      assumption
 
 lemma redex_progress : ∀ {Γ e ty}, Expr.TypeJdg Γ e ty → IsRedex e →
   CtxRespectsEnv V Γ → ∃ e', HeadSmallStep V e e' := by
-  sorry
+  intro Γ e ty e_jdg e_redex V_resp_Γ
+  cases e_redex with
+  | const =>
+    rename_i n
+    exists .value (.nat n)
+    constructor
+  | var =>
+    cases e_jdg
+    rename_i x x_ty
+    let ⟨v, ⟨v_in_V, v_jdg⟩⟩ := V_resp_Γ x ty x_ty
+    exists .value v
+    constructor
+    assumption
+  | binOp =>
+    cases e_jdg with
+    | jdg_binOp e₁_jdg e₂_jdg =>
+      rename_i v₁ v₂ op
+      cases e₁_jdg
+      cases e₂_jdg
+      rename_i v₁_jdg v₂_jdg
+      cases v₁_jdg
+      cases v₂_jdg
+      rename_i n₁ n₂
+      exists .value (.nat (op.eval n₁ n₂))
+      apply HeadSmallStep.bin_op_step rfl
+  | letInConst =>
+    rename_i x v₁ v₂
+    exists .value v₂
+    constructor
+  | funCall =>
+    rename_i v es
+    cases e_jdg with
+    | jdg_fun f_jdg es_jdg =>
+      rename_i arg_tys ret_ty
+      cases f_jdg
+      rename_i v_jdg
+      cases v_jdg
+      rename_i ps bd ps_jdg
+      exists bd.addBindings ps es sorry
+      apply HeadSmallStep.fun_step sorry rfl
 
 theorem progress {Γ : TypeContext} {ty : LLType}
   : Expr.TypeJdg Γ e ty → CtxRespectsEnv V Γ →
-    IsConst e ∨ ∃ e', SmallStep V e e' := by
+    IsValue e ∨ ∃ e', SmallStep V e e' := by
   intro e_jdg V_ext_Γ
+
   sorry
 
 -- TODO: Also interesting:
